theories/Alpha/AlphaNotILI.v
@@ -1,0 +1,54 @@
+Require Import Val Var IL RenameApart Alpha Sim.
+
+Definition alpha_ex_ili : stmt := stmtFun ((nil, stmtReturn (Var 1))::nil)
+                                     (stmtIf (Var 1)
+                                             (stmtLet 1 (Operation (Con val_false))
+                                                      (stmtApp (LabI 0) nil))
+                                             (stmtLet 1 (Operation (Con val_true))
+                                                      (stmtApp (LabI 0) nil))).
+
+Definition alpha_ex_ili_ren : stmt := stmtFun ((nil, stmtReturn (Var 1))::nil)
+                                     (stmtIf (Var 1)
+                                             (stmtLet 1 (Operation (Con val_false))
+                                                      (stmtApp (LabI 0) nil))
+                                             (stmtLet 2 (Operation (Con val_true))
+                                                      (stmtApp (LabI 0) nil))).
+
+Lemma alpha_eq
+  : alpha id id alpha_ex_ili alpha_ex_ili_ren.
+Proof.
+  repeat (econstructor; simpl; intros; inv_get; simpl).
+Qed.
+
+Example no_alpha_ili L (E:onv val) (EQ:E 1%positive = Some val_false)
+        (EQ2:E 2%positive <> Some val_one)
+  : ~ sim bot3 Sim
+      (L, E, alpha_ex_ili)
+      (L, E, alpha_ex_ili_ren).
+Proof.
+  intro.
+  eapply sim_terminate' in H as [? ?]; dcr; swap 1 2; swap 2 4.
+  - eapply star2_silent. econstructor.
+    eapply star2_silent. econstructor 4. simpl; eauto.
+    eapply val2bool_false.
+    eapply star2_silent. econstructor. reflexivity.
+    eapply star2_silent. econstructor; simpl; eauto using get.
+    simpl. eapply star2_refl.
+  - reflexivity.
+  - stuck2.
+  - inv H0. not_normal H2.
+    inv H1.
+    inv H5. simpl in *. congruence.
+    inv H4. simpl in *.
+    assert (v = val_false) by congruence. subst. rewrite val2bool_false in *. congruence.
+    inv H6. simpl in *. congruence.
+    inv H7. simpl in *.
+    inv H8. simpl in *. congruence.
+    inv H9. simpl in *. clear_trivial_eqs. simpl in *.
+    inv H10. simpl in *.
+    + assert (v = val_false) by congruence. subst.
+      lud. clear_trivial_eqs.
+      assert (val_true = val_false) by congruence.
+      eapply val_true_false_neq; eauto.
+    + inv H11.
+Qed.
